heap/tree_push.v
@@ -14,11 +14,13 @@ Local Open Scope list_scope.
 Require Import cprogs.heap.list_relation.
 Require Import cprogs.heap.definitions.
 Require Import cprogs.heap.tree_list.
+Require Import cprogs.heap.math_prop.
+Require Import cprogs.heap.tree_up.
 
 Require Import SetsClass.SetsClass.
 Local Open Scope sets.
 Import SetsNotation.
-
+(* 
 Inductive list_nth_on_partial_tree (l: list Z) (n: Z) (p: Z) (lt: partial_tree) : Prop :=
   | nth_partial_tree_nil: p = n -> lt = nil -> list_nth_on_partial_tree l n p lt
   | nth_partial_tree_cons: forall flg v t lt0, 
@@ -28,10 +30,9 @@ Inductive list_nth_on_partial_tree (l: list Z) (n: Z) (p: Z) (lt: partial_tree) 
     Znth (p / 2) l = v -> 
     list_nth_on_tree l (p + (if flg then -1 else 1)) t -> 
     list_nth_on_partial_tree l n (p / 2) lt0 -> 
-    list_nth_on_partial_tree l n p lt.
+    list_nth_on_partial_tree l n p lt. *)
 
-
-Lemma list_nth_on_partial_tree_app: forall l n p lt (flg: bool) v t,
+(* Lemma list_nth_on_partial_tree_app: forall l n p lt (flg: bool) v t,
   (if flg then
     list_nth_on_partial_tree l (n * 2 + 1) p lt /\ list_nth_on_tree l (n * 2) t /\ Znth n l = v
   else
@@ -75,6 +76,32 @@ Proof.
       injection H3; intros; subst lt0 ta va flga.
       eapply nth_partial_tree_cons; eauto.
   }
+Qed. *)
+
+Lemma tree_push_decompose_sound: forall d t v,
+  complete_tree_push d t ->
+  exists pt, t = tree_compose pt Leaf /\ complete_tree_pop d (tree_compose pt (Node v Leaf Leaf)).
+Proof.
+  intros.
+  induction H.
+  + exists nil.
+    simpl.
+    split; [tauto |].
+    apply complete_tree_pop_right_hole.
+    - apply full_tree_Leaf; lia.
+    - apply complete_tree_pop_Leaf; lia. 
+  + destruct IHcomplete_tree_push as [pt [? ?]].
+    exists (pt ++ [(true, v0, ls)]); split.
+    - rewrite tree_compose_append, H1.
+      reflexivity.
+    - rewrite tree_compose_append. 
+      apply complete_tree_pop_right_hole; tauto.
+  + destruct IHcomplete_tree_push as [pt [? ?]].
+    exists (pt ++ [(false, v0, rs)]); split.
+    - rewrite tree_compose_append, H1.
+      reflexivity.
+    - rewrite tree_compose_append. 
+      apply complete_tree_pop_left_hole; tauto. 
 Qed.
 
 Lemma full_tree_equiv1: forall d t,
@@ -172,6 +199,27 @@ Proof.
     lia.
 Qed.
 
+Lemma full_tree_next_index: forall d t, 
+  full_tree d t -> next_index (d + 1) 0 t = 0.
+Proof.
+  intros.
+  induction H; subst; simpl; auto.
+  replace (dep + 1 - 1) with dep by lia.
+  rewrite full_tree_equiv1 in H.
+  pose proof full_tree_b_dep_restrict _ _ H.
+  replace (dep - 1 + 1) with dep in H1 by lia.
+  rewrite H1; simpl.
+  replace (dep - 1 + 1) with dep in IHfull_tree1 by lia.
+  tauto.
+Qed.
+
+Lemma complete_tree_push_dep_positve: forall d t,
+  complete_tree_push d t -> 1 <= d.
+Proof.
+  intros.
+  induction H; lia.
+Qed.
+
 Lemma next_index_lowbit: forall n d t,
   complete_tree_push d t ->
   next_index d n t = n * (tree_next_pow2 d t) + next_index d 0 t.
@@ -195,13 +243,6 @@ Proof.
       specialize (IHt1 (d - 1) (n * 2) H2).
       rewrite IHt1.
       lia. 
-Qed.
-
-Lemma complete_tree_push_dep_positve: forall d t,
-  complete_tree_push d t -> 1 <= d.
-Proof.
-  intros.
-  induction H; lia.
 Qed.
 
 Lemma complete_tree_push_same_next_pow2: forall d t1 t2,
@@ -241,21 +282,7 @@ Proof.
       lia. 
 Qed.
 
-Lemma full_tree_next_index: forall d t, 
-  full_tree d t -> next_index (d + 1) 0 t = 0.
-Proof.
-  intros.
-  induction H; subst; simpl; auto.
-  replace (dep + 1 - 1) with dep by lia.
-  rewrite full_tree_equiv1 in H.
-  pose proof full_tree_b_dep_restrict _ _ H.
-  replace (dep - 1 + 1) with dep in H1 by lia.
-  rewrite H1; simpl.
-  replace (dep - 1 + 1) with dep in IHfull_tree1 by lia.
-  tauto.
-Qed.
-  
-Lemma complete_tree_next_index: forall d t,
+Lemma tree_next_index_size: forall t d,
   complete_tree_push d t ->
   next_index d 1 t = tree_size t + 1.
 Proof.
@@ -363,3 +390,239 @@ Proof.
     - constructor.
   +      
 Qed. *)
+
+Lemma list_nth_on_tree_app:  forall (l: list Z) (v n: Z) (t: tree),
+  list_nth_on_tree l n t -> list_nth_on_tree (l++[v]) n t.
+Proof.
+  intros.
+  induction H.
+  + apply list_nth_on_tree_Leaf.
+  + eapply list_nth_on_tree_Node; try tauto.
+    - rewrite Zlength_app.
+      replace (Zlength [v]) with 1 by tauto.
+      lia.
+    - rewrite app_Znth1; [tauto|lia].
+Qed.
+
+Lemma list_on_partial_tree_app: forall (l: list Z) (lt: partial_tree) (v n: Z),
+  list_on_partial_tree l n lt -> list_on_partial_tree (l ++ [v]) n lt.
+Proof.
+  intros.
+  revert n H.
+  induction lt; intros.
+  + inversion H; [|discriminate].
+    apply nil_partial_tree; tauto.
+  + destruct a as [[flg val] tr].
+    inversion H; [discriminate|].
+    injection H0; intros; subst.
+    eapply cons_partial_tree; try reflexivity; try tauto.
+    - rewrite Zlength_app.
+      replace (Zlength [v]) with 1 by tauto.
+      lia.
+    - rewrite app_Znth1; [tauto|lia].
+    - apply list_nth_on_tree_app; tauto.
+    - apply IHlt; tauto.
+Qed.
+
+Lemma list_on_tree_state_app2: forall (l: list Z) (t: tree) (lt: partial_tree) (v n  d: Z), 
+  list_on_tree_state (l,n) (lt,t) -> complete_tree_push d t ->
+  list_on_partial_tree (l++[v]) (next_index d n t) (tree_to_partial_tree_fix lt t d).
+Proof.
+  intros.
+  revert lt n d H H0.
+  induction t; intros.
+  + simpl.
+    unfold list_on_tree_state in H.
+    unfold list_on_tree_state_fix in H; simpl in H.
+    destruct H, H1, H2.
+    apply list_on_partial_tree_app; tauto.
+  + simpl.
+    remember (full_tree_b (d - 1) t1) as HQ.
+    destruct HQ; simpl.
+    - apply IHt2.
+      2: {
+        inversion H0; [tauto|].
+        pose proof full_tree_complete_tree_push _ _ H5.
+        replace (d-2+1) with (d-1) in H6 by lia.
+        tauto.
+      }
+      revert H; unfold list_on_tree_state.
+      unfold list_on_tree_state_fix; simpl; intros.
+      destruct H, H1, H2.
+      inversion H.
+      split; [tauto|].
+      split; [|tauto].
+      eapply cons_partial_tree; try reflexivity; try rewrite Odd_Div2; try lia.
+      * simpl.
+        replace (n * 2 + 1 + -1) with (n*2) by lia.
+        tauto.
+      * tauto.
+    - apply IHt1.
+      2: {
+        inversion H0; [|tauto].
+        apply full_tree_equiv1 in H3.
+        rewrite H3 in HeqHQ.
+        discriminate.
+      }
+      revert H; unfold list_on_tree_state.
+      unfold list_on_tree_state_fix; simpl; intros.
+      destruct H, H1, H2.
+      inversion H.
+      split; [tauto|].
+      split; [|tauto].
+      eapply cons_partial_tree; try reflexivity; try rewrite Even_Div2; try lia.
+      * simpl; tauto.
+      * tauto.
+Qed.
+
+(* Lemma complete_tree_holds: forall (t ts: tree) (lt: partial_tree) (d d1 v: Z), 
+  ts = (tree_compose lt t) -> complete_tree_push d ts -> complete_tree_push d1 t ->
+  (exists n, next_index d 1 ts = next_index d1 n t) ->
+  exists dep, complete_tree_pop dep (tree_compose (tree_to_partial_tree_fix lt t d1) (Node v Leaf Leaf)).
+Proof.
+  intros.
+  revert d1 t lt H H1 H2.
+  induction H0; intros.
+  + give_up.
+  + 
+Qed. *)
+
+
+Lemma complete_tree_holds: forall (t: tree)(d v: Z), 
+  complete_tree_push d t -> complete_tree_pop d (tree_compose (tree_to_partial_tree t d) (Node v Leaf Leaf)). 
+Proof.
+  intros.
+  induction H; intros.
+  + give_up.
+  + unfold tree_to_partial_tree.
+    apply full_tree_equiv1 in H.
+    simpl.
+    rewrite H. 
+  (*要写一个东西，把tree_ot_partial_tree的东西给提出来*)
+Admitted.
+
+Lemma list_on_tree_state_app: forall (l: list Z) (t: tree) (v: Z),
+  Zlength l >= 1 -> list_on_tree l t -> exists d, list_on_tree_state (l++[v], Zlength l) (tree_to_partial_tree t d,Node v Leaf Leaf).
+Proof.
+  intros.
+  unfold list_on_tree_state; simpl.
+  unfold list_on_tree_state_fix.
+  unfold list_on_tree in H0.
+  destruct H0, H1.
+  destruct H2 as [dep].
+  exists dep.
+  assert (Zlength (l ++ [v]) = Zlength l + 1). {
+    rewrite Zlength_app.
+    replace (Zlength [v]) with 1; [lia|].
+    unfold Zlength; unfold Zlength_aux; reflexivity.
+  }
+  split.
+  + eapply list_nth_on_tree_Node.
+    - rewrite H3.
+      pose proof initial_world.zlength_nonneg _ l.
+      lia.
+    - rewrite app_Znth2; [|lia].
+      replace (Zlength l - Zlength l) with 0 by lia.
+      reflexivity.
+    - eapply list_nth_on_tree_Leaf. 
+    - eapply list_nth_on_tree_Leaf. 
+  + split.
+    assert (list_on_tree_state (l, 1) (nil, t)). {
+      unfold list_on_tree_state; simpl.
+      unfold list_on_tree_state_fix.
+      split; [tauto|].
+      split; [apply nil_partial_tree; reflexivity|].
+      split; simpl; [|exists dep]; tauto.
+    }
+    pose proof list_on_tree_state_app2 l t nil v 1 dep H4 H2.
+    - replace (Zlength l) with (tree_size t + 1) by lia.
+      unfold tree_to_partial_tree.
+      rewrite <- (tree_next_index_size _ dep); tauto.
+    - split.
+      * give_up.
+      * apply complete_tree_equality.
+Admitted.
+
+Definition tree_push: tree -> Z -> tree -> Prop :=
+  fun t val t' =>
+    exists (ts: tree_state), heap_tree_up ((tree_to_partial_tree t), Node val Leaf Leaf) ts /\ t' = (tree_compose (fst ts) (snd ts)).
+
+Lemma tree_to_partial_tree_fix_hold: forall (lt: partial_tree) (t: tree),
+  MaxHeap_partial_tree lt -> MaxHeap t -> (t = Leaf \/ MaxHeap_partial_tree_v lt (get_tree_val t)) -> MaxHeap_partial_tree (tree_to_partial_tree_fix lt t).
+Proof.
+  intros.
+  revert lt H H1.
+  induction H0; intros.
+  + rewrite H.
+    simpl.
+    apply H0.
+  + subst.
+    destruct H3; [discriminate|].
+    simpl in H.
+    simpl.
+    destruct (get_snd_01 (1 + tree_size ls + tree_size rs)).
+    - apply IHMaxHeap2; [simpl; tauto|].
+      destruct H1; [left; tauto|right].
+      eapply MaxHeap_partial_tree_v_app; [reflexivity| | | | ]; tauto.
+    - apply IHMaxHeap1; [simpl; tauto|].
+      destruct H0; [left; tauto|right].
+      eapply MaxHeap_partial_tree_v_app; [reflexivity| | | | ]; tauto.
+Qed.
+
+Lemma MaxHeap_impl_MaxHeap_tree_up: forall (t: tree) (v: Z),
+  MaxHeap t -> MaxHeap_tree_up (tree_to_partial_tree t,Node v Leaf Leaf).
+Proof.
+  intros.
+  revert H.
+  induction t; intros.
+  + unfold tree_to_partial_tree.
+    unfold MaxHeap_tree_up.
+    simpl.
+    split; [tauto|].
+    split.
+    - eapply MaxHeap_Node; [reflexivity| | | | ]; tauto.
+    - exists v, Leaf, Leaf.
+      tauto.
+  + unfold MaxHeap_tree_up.
+    unfold fst, snd.
+    inversion H; [discriminate|].
+    injection H0; intros; subst.
+    specialize (IHt1 H1).
+    specialize (IHt2 H2).
+    split.
+    2: {
+      split; [|exists v, Leaf, Leaf; tauto].
+      eapply MaxHeap_Node; [reflexivity| | | |]; try tauto.
+      apply MaxHeap_Leaf; reflexivity.
+      apply MaxHeap_Leaf; reflexivity.
+    }
+    unfold tree_to_partial_tree.
+    apply tree_to_partial_tree_fix_hold; [unfold MaxHeap_partial_tree; tauto|tauto|right].
+    apply MaxHeap_partial_tree_v_nil; reflexivity.
+Qed.
+
+Lemma Push_tree_list_rel: forall (l l': list Z) (t: tree) (v: Z),
+  list_on_tree l t -> heap_push l v l' -> MaxHeap t ->
+  exists t', list_on_tree l' t' /\ MaxHeap t' /\ tree_push t v t'.
+Proof.
+  intros.
+  assert (Zlength l >= 1). {
+    unfold list_on_tree in H.
+    inversion H; lia.
+  }
+  unfold heap_push in H0.
+  destruct H0.
+  pose proof list_on_tree_state_app _ _ v H2 H.
+  pose proof MaxHeap_impl_MaxHeap_tree_up _ v H1.
+  pose proof Up_tree_list_rel _ _ _ H3 H0 H4.
+  destruct H5 as [t'].
+  destruct H5, H6.
+  pose proof list_on_tree_state_impl_tree_compose _ _ H6.
+  simpl fst in H8.
+  exists (tree_compose (fst t') (snd t')).
+  split; [tauto|].
+  split; [tauto|].
+  unfold tree_push.
+  exists t'.
+  tauto.
+Qed.
