heap/tree_up.v
@@ -1,0 +1,548 @@
+Require Import FloydSeq.proofauto.
+(* Require Import cprogs.heap.program. *)
+Require Import Notations Logic Datatypes.
+From Coq Require Import String List ZArith. 
+From compcert Require Import Coqlib Integers Floats AST Ctypes Cop Clight Clightdefs.
+Require Import Coq.Logic.Classical_Pred_Type.
+Require Import Coq.Logic.Classical_Prop.
+
+Require Import Coq.micromega.Psatz.
+Local Open Scope string.
+Local Open Scope nat_scope.
+Local Open Scope Z_scope.
+Local Open Scope list_scope.
+Require Import cprogs.heap.list_relation.
+Require Import cprogs.heap.definitions.
+Require Import cprogs.heap.tree_list.
+Require Import cprogs.heap.math_prop.
+
+Require Import SetsClass.SetsClass.
+Local Open Scope sets.
+Import SetsNotation.
+
+Definition tree_up_succeed:
+  tree_state -> tree_state -> Prop:=
+    fun t1 t2 => exists t3 l', 
+    (t3::l' = (fst t1)) /\ (l' = (fst t2)) /\
+    (exists v ls rs, (swap_up_and_combine v ls rs t3) = (snd t2) /\ (snd t1) = (Node v ls rs)) /\ 
+    ((get_tree_val (snd t1)) > (snd (fst t3))).
+
+Definition tree_up_fail:
+  tree_state -> tree_state -> Prop:=
+    Rels.test(fun t => 
+      match (fst t) with
+      | nil => True
+      | t2::lt => snd (fst t2) >= (get_tree_val (snd t))
+      end).
+
+Definition heap_tree_up:
+  tree_state -> tree_state -> Prop:=
+  (clos_refl_trans tree_up_succeed) ∘ tree_up_fail.
+
+Definition MaxHeap_tree_up(ts: tree_state): Prop :=
+  MaxHeap_partial_tree (fst ts) /\ MaxHeap (snd ts) /\ (exists v ls rs, snd ts = Node v ls rs /\ 
+  (ls = Leaf \/ MaxHeap_partial_tree_v (fst ts) (get_tree_val ls)) /\ 
+  (rs = Leaf \/ MaxHeap_partial_tree_v (fst ts) (get_tree_val rs))).
+
+Lemma swap_up_right_hold_true: forall (l l': list_state) (ls rs tr: tree) (v1 v2: Z) (lt: partial_tree),
+  list_on_tree_state l ((true,v2,tr) :: lt, Node v1 ls rs) -> list_relation.list_swap (snd l) (snd l') (fst l) (fst l') -> snd l / 2 = snd l' -> list_on_tree_state l' (lt, Node v1 tr (Node v2 ls rs)).
+Proof.
+  unfold list_on_tree_state.
+  unfold list_on_tree_state_fix.
+  destruct l as [l n].
+  destruct l' as [l' n'].
+  simpl; intros; subst.
+  destruct H, H1.
+  inversion H1; [discriminate |].
+  apply cons_inv in H3; destruct H3.
+  inversion H2; subst; clear H2.
+  assert (1 <= n / 2 < n). {
+    split.
+    + lia.
+    + apply Div_2_gt_0.
+      lia. 
+  }
+  inversion H.
+  pose proof list_swap_rela_rewrite l l' n (n / 2) ltac:(lia) ltac:(lia) H0.
+  subst; clear H0.
+  split.
+  + eapply list_nth_on_tree_Node; eauto.
+    - rewrite list_swap_Zlength by lia; lia.
+    - unfold list_swap.
+      rewrite upd_Znth_diff.
+      * rewrite upd_Znth_same; [auto | lia].
+      * rewrite upd_Znth_Zlength by lia; lia.
+      * rewrite upd_Znth_Zlength by lia; lia.
+      * lia.
+    - injection H3; intros; subst.
+      replace (n / 2 * 2) with (n + -1) by lia. 
+      unfold list_swap.
+      apply list_nth_on_tree_upd.
+      * apply list_nth_on_tree_upd; [auto | lia |].
+        apply less_is_not_child_index; lia.
+      * rewrite upd_Znth_Zlength by lia; lia.
+      * apply rchild_is_not_lchild with (pp := n / 2); [lia | lia |].
+        apply is_child_index_self; auto.
+    - injection H3; intros; subst.
+      rewrite <- H5.
+      eapply list_nth_on_tree_Node.
+      * rewrite list_swap_Zlength by lia; lia.
+      * unfold list_swap.
+        rewrite upd_Znth_same; [reflexivity | ].
+        rewrite upd_Znth_Zlength by lia; lia.
+      * unfold list_swap.
+        apply list_nth_on_tree_upd.
+        -- apply list_nth_on_tree_upd; [auto | lia |].
+           apply less_is_not_child_index; lia.
+        -- rewrite upd_Znth_Zlength by lia; lia.
+        -- apply less_is_not_child_index; lia.
+      * unfold list_swap.
+        apply list_nth_on_tree_upd.
+        -- apply list_nth_on_tree_upd; [auto | lia |].
+           apply less_is_not_child_index; lia.
+        -- rewrite upd_Znth_Zlength by lia; lia.
+        -- apply less_is_not_child_index; lia.
+  + split.
+    inversion H8; subst.
+    - eapply nil_partial_tree; eauto.
+    - pose proof Z.div_lt_upper_bound (n / 2) 2 (n / 2) ltac:(lia) ltac:(lia).
+      pose proof Z.div_le_lower_bound (n / 2) 2 1 ltac:(lia) ltac:(lia).
+      eapply cons_partial_tree. eauto.
+      * rewrite list_swap_Zlength by lia; lia. 
+      * unfold list_swap.
+        tauto.
+      * unfold list_swap.
+        rewrite upd_Znth_diff.
+        -- rewrite upd_Znth_diff by lia; reflexivity.
+        -- rewrite upd_Znth_Zlength by lia; lia.
+        -- rewrite upd_Znth_Zlength by lia; lia.
+        -- lia.
+      * inversion H3; subst.
+        unfold list_swap.
+        apply list_nth_on_tree_upd.
+        -- apply list_nth_on_tree_upd; [auto | lia |].
+           destruct flg0.
+           ++ apply rchild_is_not_lchild with (pp := n / 2 / 2); [lia | lia |].
+              apply is_child_index_self; auto.
+           ++ apply less_is_not_child_index; lia. 
+        -- rewrite upd_Znth_Zlength by lia; lia.
+        -- destruct flg0.
+           ++ apply rchild_is_not_lchild with (pp := n / 2 / 2); [lia | lia |].
+              apply is_child_index_gp; [lia | apply is_child_index_self; auto].
+           ++ apply lchild_is_not_rchild with (pp := n / 2 / 2); [lia | lia |].
+              apply is_child_index_gp; [lia | apply is_child_index_self; auto].
+      * apply list_on_partial_tree_upd.
+        -- rewrite upd_Znth_Zlength by lia; lia.
+        -- rewrite upd_Znth_Zlength by lia; lia.
+        -- apply is_child_index_gp; [lia | ].
+           apply is_child_index_gp; [lia | apply is_child_index_self; auto].
+        -- apply list_on_partial_tree_upd; [lia | lia | |auto].
+           apply is_child_index_gp; [lia | apply is_child_index_self; auto].
+    - assert (tree_same (Node (Znth n l) tr (Node v2 ls rs)) (Node v2 tr (Node (Znth n l) ls rs))). {
+      apply Node_same; [apply tree_same_rel; reflexivity|].
+      apply Node_same; apply tree_same_rel; reflexivity.
+    }
+      split.
+      * rewrite list_swap_Zlength by lia.
+        rewrite <- H10.
+        apply tree_same_size.
+        apply tree_compose_same.
+        apply H0.
+      * destruct H11 as [dep].
+        exists dep.
+        apply (tree_same_complete_tree (tree_compose lt0 (Node v2 tr (Node (Znth n l) ls rs)))); [|tauto].
+        apply tree_compose_same.
+        apply tree_same_swap.
+        apply H0.
+Qed.
+
+Lemma swap_up_left_hold_true: forall (l l': list_state) (ls rs tr: tree) (v1 v2: Z) (lt: partial_tree),
+  list_on_tree_state l ((false,v2,tr) :: lt, Node v1 ls rs) -> list_relation.list_swap (snd l) (snd l') (fst l) (fst l') -> snd l / 2 = snd l' -> list_on_tree_state l' (lt, (Node v1 (Node v2 ls rs) tr)).
+Proof.
+  unfold list_on_tree_state.
+  unfold list_on_tree_state_fix.
+  destruct l as [l n].
+  destruct l' as [l' n'].
+  simpl; intros; subst.
+  destruct H, H1.
+  inversion H1; [discriminate |].
+  apply cons_inv in H3; destruct H3.
+  inversion H2; subst; clear H2.
+  assert (1 <= n / 2 < n). {
+    split.
+    + lia.
+    + apply Div_2_gt_0.
+      lia. 
+  }
+  inversion H.
+  inversion H5.
+  pose proof list_swap_rela_rewrite l l' n (n / 2) ltac:(lia) ltac:(lia) H0.
+  subst; clear H0.
+  split.
+  + eapply list_nth_on_tree_Node; eauto.
+    - rewrite list_swap_Zlength by lia; rewrite <- H17; lia.
+    - unfold list_swap.
+      rewrite upd_Znth_diff; try rewrite <- H17.
+      * rewrite upd_Znth_same; [auto | lia].
+      * rewrite upd_Znth_Zlength by lia; lia.
+      * rewrite upd_Znth_Zlength by lia; lia.
+      * lia.
+    - injection H3; intros; subst.
+      rewrite <- H5.
+      replace (n / 2 * 2) with (n) by lia. 
+      eapply list_nth_on_tree_Node.
+      * rewrite list_swap_Zlength by lia; lia.
+      * unfold list_swap.
+        rewrite upd_Znth_same; [reflexivity | ].
+        rewrite upd_Znth_Zlength by lia; lia.
+      * unfold list_swap.
+        apply list_nth_on_tree_upd.
+        -- apply list_nth_on_tree_upd; [auto | lia |].
+           apply less_is_not_child_index; lia.
+        -- rewrite upd_Znth_Zlength by lia; lia.
+        -- apply less_is_not_child_index; lia.
+      * unfold list_swap.
+        apply list_nth_on_tree_upd.
+        -- apply list_nth_on_tree_upd; [auto | lia |].
+           apply less_is_not_child_index; lia.
+        -- rewrite upd_Znth_Zlength by lia; lia.
+        -- apply less_is_not_child_index; lia. 
+    - inversion H3; subst.
+      replace (n / 2 * 2 + 1) with (n + 1) by lia.
+      unfold list_swap.
+      apply list_nth_on_tree_upd.
+      * apply list_nth_on_tree_upd; [auto | lia |].
+        rewrite <- H5.
+        replace (n / 2 * 2) with n by lia.
+        apply H7.
+        apply less_is_not_child_index.
+        rewrite <- H5.
+        lia.
+      * rewrite upd_Znth_Zlength by lia; lia.
+      * rewrite <- H17. 
+        apply lchild_is_not_rchild with (pp := n / 2); [lia | lia |].
+        apply is_child_index_self; auto.
+        lia.
+  + split. inversion H8; subst.
+    - eapply nil_partial_tree; eauto.
+      rewrite <- H17.
+      lia.
+    - pose proof Z.div_lt_upper_bound (n / 2) 2 (n / 2) ltac:(lia) ltac:(lia).
+      pose proof Z.div_le_lower_bound (n / 2) 2 1 ltac:(lia) ltac:(lia).
+      eapply cons_partial_tree; eauto.
+      * rewrite list_swap_Zlength by lia; rewrite <- H17; lia. 
+      * unfold list_swap.
+        rewrite <- ! H17.
+        rewrite <- ! H9.
+        lia.
+      * unfold list_swap.
+        rewrite <- H17.
+        rewrite upd_Znth_diff.
+        -- rewrite upd_Znth_diff by lia; reflexivity.
+        -- rewrite upd_Znth_Zlength by lia; lia.
+        -- rewrite upd_Znth_Zlength by lia; lia.
+        -- lia.
+      * apply list_nth_on_tree_upd.
+        -- apply list_nth_on_tree_upd; [auto | lia |].
+           destruct flg0; rewrite <- H17; tauto.
+           destruct flg0; rewrite <- H17.
+           ++ apply rchild_is_not_lchild with (pp := n / 2 / 2); [lia | lia |].
+           apply is_child_index_self; auto.
+           ++ apply less_is_not_child_index; lia. 
+        -- rewrite upd_Znth_Zlength by lia; lia.
+        -- destruct flg0; rewrite <- H17.
+           ++ apply rchild_is_not_lchild with (pp := n / 2 / 2); [lia | lia |].
+              apply is_child_index_gp; [lia | apply is_child_index_self; auto].
+           ++ apply lchild_is_not_rchild with (pp := n / 2 / 2); [lia | lia |].
+              apply is_child_index_gp; [lia | apply is_child_index_self; auto].
+      * unfold list_swap.
+        apply list_on_partial_tree_upd; try rewrite <- H17.
+        -- rewrite upd_Znth_Zlength by lia; lia.
+        -- rewrite upd_Znth_Zlength by lia; lia.
+        -- apply is_child_index_gp; [lia | ].
+           apply is_child_index_gp; [lia | apply is_child_index_self; auto].
+        -- apply list_on_partial_tree_upd; [lia | lia | |auto].
+           apply is_child_index_gp; [lia | apply is_child_index_self; auto].
+     - assert (tree_same (Node (Znth n l) (Node v2 ls rs) tr) (Node v2 (Node (Znth n l) ls rs) tr)). {
+      apply Node_same; [|apply tree_same_rel; reflexivity].
+      apply Node_same; apply tree_same_rel; reflexivity.
+    }
+      split.
+      * rewrite list_swap_Zlength by lia.
+        rewrite <- H10.
+        apply tree_same_size.
+        apply tree_compose_same.
+        apply H0.
+      * destruct H11 as [dep].
+        exists dep.
+        apply (tree_same_complete_tree (tree_compose lt0 (Node v2 (Node (Znth n l) ls rs) tr))); [|tauto].
+        apply tree_compose_same.
+        apply tree_same_swap.
+        apply H0.
+Qed.
+
+Lemma Up_tree_list_succeed: forall (l l': list_state) (t: tree_state),
+  list_on_tree_state l t -> list_up_succeed l l' -> MaxHeap_tree_up t ->
+  exists t', tree_up_succeed t t' /\ list_on_tree_state l' t' /\ MaxHeap_tree_up t'.
+Proof.
+  intros.
+  unfold list_up_succeed in H0.
+  destruct H0, H2, H3, H4, H5.
+  pose proof list_on_tree_state_impl_up_val _ _ H H0 ltac:(lia).
+  destruct H7 as [lt [v [tr [flg]]]].
+  destruct H7, H8.
+  pose proof legal_list_impl_legal_tree_state _ _ H H0.
+  unfold legal_tree_state in H10.
+  destruct H10 as [v2 [ls [rs]]].
+  rewrite H4 in H5.
+  unfold get_list_val in H9; simpl in H9.
+  rewrite H10 in H8; unfold get_tree_val in H8.
+  assert (v2 > v) by lia.
+  destruct flg.
+  + exists (lt, (Node v2 tr (Node v ls rs))).
+    split.
+    - unfold tree_up_succeed.
+      exists (true, v, tr), lt.
+      split; [tauto|].
+      split; [tauto|].
+      split; [|rewrite H10; simpl; lia].
+      exists v2, ls, rs.
+      split; [|tauto].
+      unfold swap_up_and_combine; simpl.
+      reflexivity.
+    - split.
+      * eapply swap_up_right_hold_true; eauto.
+        rewrite H7, <- H10.
+        auto.
+      * unfold MaxHeap_tree_up; simpl.
+        unfold MaxHeap_tree_up in H1.
+        destruct H1.
+        rewrite <- H7 in H1.
+        unfold MaxHeap_partial_tree in H1.
+        destruct H1, H13.
+        split; [apply (MaxHeap_partial_tree_v_impl _ _ H14)|].
+        destruct H12.
+        destruct H15 as [v3 [ls2 [rs2]]].
+        rewrite H10 in H12; simpl in H12.
+        destruct H15.
+        rewrite H10 in H15.
+        injection H15; intros; subst.
+        split. destruct H13.
+        ++ eapply MaxHeap_Node; [ reflexivity |apply H1 | |left; tauto|right; unfold get_tree_val; lia].
+           destruct H16.
+           inversion H12;[discriminate|].
+           injection H16; intros; subst.
+           eapply MaxHeap_Node; [reflexivity| | | | ]; try tauto.
+           destruct H9; [left; tauto|].
+           inversion H8; rewrite H9 in H7; [discriminate|].
+           injection H7; intros; subst.
+           right; lia.
+           destruct H13; [left; tauto|]. inversion H8; rewrite H13 in H7; [discriminate|].
+           injection H7; intros; subst.
+           right; lia.
+        ++ eapply MaxHeap_Node;[reflexivity|apply H1| | right; lia| right; unfold get_tree_val; lia].
+           destruct H16.
+           inversion H12;[discriminate|].
+           injection H16; intros; subst.
+           eapply MaxHeap_Node; [reflexivity| | | | ]; try tauto.
+           destruct H9; [left; tauto|].
+           inversion H9; rewrite H21 in H7; [discriminate|].
+           injection H7; intros; subst.
+           right; lia.
+           destruct H13; [left; tauto|].
+           inversion H13; rewrite H21 in H7; [discriminate|].
+           injection H7; intros; subst.
+           right; lia.
+        ++ exists (get_list_val l), tr, (Node (Znth (snd l / 2) (fst l)) ls2 rs2); simpl.
+           split; [reflexivity|].
+           split; [|right; tauto].
+           destruct H13; [left; tauto|right].
+           apply (MaxHeap_partial_tree_v_change_v _ _ _ H14 H8).
+  + exists (lt, (Node v2 (Node v ls rs) tr)).
+    split.
+    - unfold tree_up_succeed.
+      exists (false, v, tr), lt.
+      split; [tauto|].
+      split; [tauto|].
+      split; [|rewrite H10; simpl; lia].
+      exists v2, ls, rs.
+      split; [|tauto].
+      unfold swap_up_and_combine; simpl.
+      reflexivity.
+    - split.
+      * eapply swap_up_left_hold_true; eauto.
+        rewrite H7, <- H10.
+        auto.
+      * unfold MaxHeap_tree_up. simpl.
+        unfold MaxHeap_tree_up in H1.
+        destruct H1.
+        rewrite <- H7 in H1.
+        unfold MaxHeap_partial_tree in H1.
+        destruct H1, H13.
+        split; [apply (MaxHeap_partial_tree_v_impl _ _ H14)|].
+        destruct H12.
+        destruct H15 as [v3 [ls2 [rs2]]].
+        rewrite H10 in H12; simpl in H12.
+        destruct H15.
+        rewrite H10 in H15.
+        injection H15; intros; subst.
+        split. destruct H13.
+        ++ eapply MaxHeap_Node; [ reflexivity | |apply H1 |right; unfold get_tree_val; lia|left; tauto].
+           destruct H16.
+           inversion H12;[discriminate|].
+           injection H16; intros; subst.
+           eapply MaxHeap_Node; [reflexivity| | | | ]; try tauto.
+           destruct H9; [left; tauto|].
+           inversion H8; rewrite H9 in H7; [discriminate|].
+           injection H7; intros; subst.
+           right; lia.
+           destruct H13; [left; tauto|]. inversion H8; rewrite H13 in H7; [discriminate|].
+           injection H7; intros; subst.
+           right; lia.
+        ++ eapply MaxHeap_Node; [ reflexivity | |apply H1 |right; unfold get_tree_val; lia|right; lia].
+           destruct H16.
+           inversion H12;[discriminate|].
+           injection H16; intros; subst.
+           eapply MaxHeap_Node; [reflexivity| | | | ]; try tauto.
+           destruct H9; [left; tauto|].
+           inversion H9; rewrite H21 in H7; [discriminate|].
+           injection H7; intros; subst.
+           right; lia.
+           destruct H13; [left; tauto|].
+           inversion H13; rewrite H21 in H7; [discriminate|].
+           injection H7; intros; subst.
+           right; lia.
+        ++ exists (get_list_val l), (Node (Znth (snd l / 2) (fst l)) ls2 rs2), tr; simpl.
+           split; [reflexivity|].
+           split; [right; tauto |].
+           destruct H13; [left; tauto|right].
+           apply (MaxHeap_partial_tree_v_change_v _ _ _ H14 H8).
+Qed.
+
+Lemma Up_tree_list_succeed_clos_refl_trans: forall (l l': list_state) (t: tree_state),
+  list_on_tree_state l t -> (clos_refl_trans list_up_succeed) l l' -> MaxHeap_tree_up t ->
+  exists t', (clos_refl_trans tree_up_succeed) t t' /\ list_on_tree_state l' t' /\ MaxHeap_tree_up t'.
+Proof.
+  intros.
+  revert t H H1.
+  induction_1n H0.
+  + exists t.
+    split; [|tauto].
+    exists 0%nat.
+    unfold nsteps.
+    reflexivity.
+  + pose proof Up_tree_list_succeed _ _ _ H H2 H1.
+    destruct H3 as [t'].
+    destruct H3; destruct H4.
+    specialize (IHrt _ H4 H5).
+    destruct IHrt as [t'0].
+    exists t'0.
+    destruct H6, H7.
+    split; [|tauto].
+    etransitivity_1n; [apply H3|apply H6].
+Qed.
+
+Lemma Up_tree_list_fail: forall (l: list_state) (t: tree_state),
+  list_on_tree_state l t -> list_up_fail l l ->
+  tree_up_fail t t.
+Proof.
+  intros.
+  unfold list_up_fail in H0.
+  destruct t as [lt t].
+  revert H0; unfold_RELS_tac; intros.
+  destruct H0; clear H1.
+  destruct H0, H1.
+  + pose proof list_on_tree_state_impl_all _ _  H ltac:(lia).
+    simpl in H2.
+    unfold tree_up_fail; unfold_RELS_tac.
+    simpl.
+    split; [|reflexivity].
+    destruct lt; [tauto|discriminate].
+  + destruct H1.
+    pose proof list_on_tree_state_impl_up_val _ _ H H0 ltac:(lia).
+    destruct H3 as [lt0].
+    destruct H3, H3, H3, H3, H4.
+    unfold tree_up_fail; unfold_RELS_tac.
+    split; [|reflexivity].
+    simpl; destruct lt; [discriminate|].
+    simpl in H4.
+    rewrite H4.
+    simpl in H3.
+    destruct p as [[flg v] tr]; subst.
+    simpl.
+    unfold get_list_val in H3.
+    simpl in H3.
+    injection H3.
+    intros.
+    lia.
+Qed.
+
+Lemma Up_fail_impl_MaxHeap: forall (t: tree_state),
+  tree_up_fail t t -> MaxHeap_tree_up t -> MaxHeap (tree_compose (fst t) (snd t)).
+Proof.
+  intros.
+  destruct t as [lt t].
+  unfold tree_up_fail in H.
+  revert H; unfold_RELS_tac; intros.
+  simpl in H.
+  destruct lt.
+  + simpl.
+    unfold MaxHeap_tree_up in H0.
+    tauto.
+  + destruct p as [[flg val] t2 ].
+    simpl in H.
+    simpl fst; simpl snd.
+    destruct H; clear H1.
+    unfold MaxHeap_tree_up in H0.
+    simpl in H0.
+    destruct H0, H0, H2.
+    assert (MaxHeap_partial_tree ((flg, val, t2) :: lt)). {
+      unfold MaxHeap_partial_tree.
+      split; tauto.
+    }
+    destruct t.
+    - pose proof MaxHeap_partial_tree_v_impl _ _ H3.
+      destruct H1.
+      apply (tree_compose_MaxHeap ((flg, val, t2) :: lt) Leaf H1 ltac:(tauto)).
+    - assert (MaxHeap_partial_tree_v ((flg, val, t2) :: lt) v). {
+        eapply MaxHeap_partial_tree_v_app; [reflexivity| | | | ]; try tauto.
+        simpl in H.
+        lia.
+      }
+      destruct H1.
+      apply (tree_compose_MaxHeap ((flg, val, t2) :: lt) (Node v t1 t3) H1 ltac:(tauto)).
+Qed.
+
+Lemma list_up_fail_impl_eq: forall (l l': list_state),
+  list_up_fail l l' -> l = l'.
+Proof.
+  intros; revert H.
+  unfold list_up_fail.
+  unfold_RELS_tac.
+  tauto.
+Qed.
+
+Lemma Up_tree_list_rel: forall (l l': list_state) (t: tree_state),
+  list_on_tree_state l t -> heap_list_up l l' -> MaxHeap_tree_up t ->
+  exists t', heap_tree_up t t' /\ list_on_tree_state l' t' /\ MaxHeap (tree_compose (fst t') (snd t')).
+Proof.
+  intros.
+  unfold heap_list_up in H0.
+  revert H0; unfold_RELS_tac; intros.
+  destruct H0 as [l1]; destruct H0.
+  pose proof Up_tree_list_succeed_clos_refl_trans _ _ _ H H0 H1.
+  pose proof list_up_fail_impl_eq _ _ H2.
+  subst.
+  destruct H3 as [t'].
+  destruct H3, H4.
+  exists t'.
+  split.
+  pose proof Up_tree_list_fail _ _ H4 H2.
+  + unfold heap_tree_up.
+    unfold_RELS_tac.
+    exists t'.
+    tauto.
+  + split;[tauto|].
+    pose proof Up_tree_list_fail _ _ H4 H2.
+    apply (Up_fail_impl_MaxHeap _ H6 H5).
+Qed.
